Cslib/Computability/Machines/MultiTapeTuring/Routines/ListOps.lean
@@ -22,18 +22,28 @@ public def pushList {k : ℕ} (d : Data) (i : Fin k) : MultiTapeTM k Char :=
 
 /-- Remove the first element from a list encoding on tape `i`.
     Running `popEnc` on an empty list does not modify the tape. -/
+public def popList {k : ℕ} (i : Fin k) : MultiTapeTM k Char := sorry
+
+/-- Remove the first element from a list encoding on tape `i`.
+    Running `popEnc` on an empty list does not modify the tape. -/
 public def popEnc {k : ℕ} (i : Fin k) : MultiTapeTM k Char := sorry
 
 /-- `pushList d i` prepends a Data element to the topmost `Data.list` on tape `i`. -/
 @[simp]
 public lemma pushList_eval_struct {k : ℕ} {d : Data} {i : Fin k}
-    {views : Fin k → TapeView}
-    {ds : List Data}
-    (h_path : (views i).path = [])
-    (h_data : (views i).data = Data.list ds) :
+    {views : Fin k → TapeView} :
     (pushList d i).eval_struct views = some
-      (Function.update views i
-        ⟨Data.list (d :: ds), []⟩) := by sorry
+      (Function.update views i (match views i with
+        | ⟨Data.list ds, []⟩ => ⟨Data.list (d :: ds), []⟩
+        | _ => views i)) := by sorry
+
+@[simp]
+public lemma popList_eval_struct {k : ℕ} {i : Fin k}
+    {views : Fin k → TapeView} :
+    (popList i).eval_struct views = some
+      (Function.update views i (match views i with
+        | ⟨Data.list (d :: ds), []⟩ => ⟨Data.list ds, []⟩
+        | _ => views i)) := by sorry
 
 /-- `popEnc i` removes the first element from the topmost `Data.list` on tape `i`. -/
 @[simp]
